src/AST.v
@@ -7,6 +7,7 @@ Require Import Coqlib.
 Require Import Bitvectors.
 Require Import Builtins.
 
+
 (* An identifier is both a unique identifier and a name, but the name is meaningless *)
 Definition ident : Type := Z * string.
 
